cedar-lean/Cedar/Thm/SymCC/Opt/CompiledPolicies.lean
@@ -57,11 +57,11 @@ theorem intoCompiledPolicies_correctness {p : Policy} {Γ : Validation.TypeEnv} 
   simp [Opt.isAuthorized, Opt.satisfiedPolicies, Opt.compileWithEffect]
   cases p'.effect <;> simp [Factory.anyTrue, Factory.or, Factory.not, Factory.and]
   all_goals {
-    cases h : Opt.compile p'.toExpr (SymEnv.ofEnv Γ) <;> simp [Data.Set.mapUnion_empty]
+    cases h : Opt.compile p'.toExpr (SymEnv.ofEnv Γ) <;> simp [List.mapUnion_nil]
     have hwf := Opt.compile_footprint_wf h
-    simp [EmptyCollection.emptyCollection, Data.Set.union_empty_right Data.Set.mapUnion_wf, Data.Set.union_empty_left Data.Set.mapUnion_wf]
-    rw [Data.Set.mapUnion_cons (by simp [hwf])]
-    simp [Data.Set.mapUnion_empty, EmptyCollection.emptyCollection, Data.Set.union_empty_right hwf]
+    simp [EmptyCollection.emptyCollection, Data.Set.union_empty_right List.mapUnion_wf, Data.Set.union_empty_left List.mapUnion_wf]
+    rw [List.mapUnion_cons (by simp [hwf])]
+    simp [List.mapUnion_nil, EmptyCollection.emptyCollection, Data.Set.union_empty_right hwf]
   }
 
 /--
